src/Qafny/Env.hs
@@ -69,14 +69,14 @@ initTState = TState
 
 
 data SplitScheme = SplitScheme
-  { schROrigin     :: Range -- the original range
-  , schRTo         :: Range -- the range splitted _to_
-  , schRsRem       :: [Range] -- the remainder range
-  , schQty         :: QTy     -- entanglement types
-  , schSMain       :: STuple  -- the partition that was splitted _from_
-  --  , schSAux    :: STuple  -- the partition that was splitted _to_
-  , schVEmitOrigin :: Var   -- the emit variable of the original range
-  , schVsEmitAll   :: [Var] -- the emit variables of new ranges
+  { schROrigin     :: Range   -- | the original range
+  , schRTo         :: Range   -- | the range splitted _to_
+  , schRsRem       :: [Range] -- | the remainder range
+  , schQty         :: QTy     -- | entanglement types
+  , schSMain       :: STuple  -- | the partition that was splitted _from_
+  --  , schSAux    :: STuple  -- | the partition that was splitted _to_
+  , schVEmitOrigin :: Var     -- | the emit variable of the original range
+  , schVsEmitAll   :: [Var]   -- | the emit variables of new ranges
   }
   deriving Show
 
@@ -87,4 +87,6 @@ data CastScheme = CastScheme
   , schTNewEmit  :: Ty
   , schQtOld     :: QTy
   , schQtNew     :: QTy
+  , schRsCast    :: [Range] -- | casted ranges
   }
+  deriving Show
