src/Qafny/TypeUtils.hs
@@ -10,3 +10,9 @@ typingQEmit TEN   = TSeq TNat
 typingQEmit TEN01 = TSeq (TSeq TNat)
 {-# INLINE typingQEmit #-}
 
+
+-- | Check if the given type is an 'EN'-like type.
+isEN :: QTy -> Bool
+isEN TEN01 = True
+isEN TEN   = True
+isEN _     = False
