external/QPreludeUntyped.dfy
@@ -1,12 +1,12 @@
-// include "libraries/src/NonlinearArithmetic/Power2.dfy"
 // TODO: study what the `LittleEndianNatConversions` is
 // include "libraries/src/Collections/Sequences/LittleEndianNatConversions.dfy"
 include "libraries/src/Collections/Sequences/LittleEndianNat.dfy"
 include "libraries/src/Collections/Sequences/Seq.dfy"
+include "libraries/src/NonlinearArithmetic/Power2.dfy"
 
 abstract module {:options "-functionSyntax:4"} QPreludeUntyped {
   import opened LittleEndianNat
-  // import opened Seq
+  import opened Power2
   import opened Seq
 
   // import opened Seq
@@ -24,6 +24,29 @@ abstract module {:options "-functionSyntax:4"} QPreludeUntyped {
 
   function CastNorCH01(q : seq<nat>) : (c : seq<seq<nat>>)
     requires forall k : nat | k < |q| :: q[k] == 0 || q[k] == 1
-    ensures c == [q]
+    ensures c ==  [q]
   ;
+
+  // (|0⟩ + α|1⟩) ⊗ (|0⟩ + α|1⟩) ⊗ (|0⟩ + β|1⟩)
+  // |0, 0, 0⟩ + α|1, 0, 0⟩ + ...
+  //
+  function CastHadTEN01(q : seq<int>) : (c : seq<seq<nat>>)
+    requires forall k : nat | k < |q| :: q[k] == 0 || q[k] == -1
+    ensures |c| == Pow2(|q|) && forall i : nat | i < |c| :: |c[i]| == |q|
+    ensures forall i : nat | i < Pow2(|q|) :: 
+            forall j : nat | j < |q| :: Locate(i, j) == c[i][j]
+  ;
+
+  function CastHadTEN01'1(q : seq<int>) : (c : seq<seq<nat>>)
+    requires |q| == 1
+    requires forall k : nat | k < |q| :: q[k] == 0 || q[k] == -1
+    ensures c == [[0], [1]]
+  ;
+
+
+  function Locate(i : nat, j : nat) : nat
+  {
+    if i % Pow2(j + 1) < Pow2(j) then 0 else 1
+  }
+            
 }
